src/Std/Data/TreeMap/Raw/Lemmas.lean
@@ -2012,6 +2012,21 @@ theorem isEmpty_inter_iff [TransCmp cmp] (h₁ : t₁.WF) (h₂ : t₂.WF) :
 
 end Inter
 
+section
+variable {β : Type v} {m₁ m₂ : Raw α β cmp}
+
+theorem Const.Equiv.beq [TransCmp cmp] [BEq β] [ReflBEq β] (h₁ : m₁.WF) (h₂ : m₂.WF) : m₁ ~m m₂ → m₁ == m₂ :=
+  fun h => DTreeMap.Raw.Const.Equiv.beq h₁ h₂ h.1
+
+theorem Const.Equiv_of_beq_eq_true [TransCmp cmp] [LawfulEqCmp cmp] [BEq β] [LawfulBEq β] (h₁ : m₁.WF) (h₂ : m₂.WF) : m₁ == m₂ → m₁ ~m m₂ :=
+  fun hyp => ⟨@DTreeMap.Raw.Const.Equiv_of_beq_eq_true α _ β m₁.1 m₂.1 _ _ _ _ h₁.1 h₂.1 hyp⟩
+
+theorem Const.Equiv.beq_congr [TransCmp cmp] [LawfulEqCmp cmp] [BEq β] {m₃ m₄ : Raw α β cmp} (h₁ : m₁.WF) (h₂ : m₂.WF) (h₃ : m₃.WF) (h₄ : m₄.WF) :
+    m₁ ~m m₃ → m₂ ~m m₄ → (m₁ == m₂) = (m₃ == m₄) :=
+  fun w1 w2 => DTreeMap.Raw.Const.Equiv.beq_congr h₁ h₂ h₃ h₄ w1.1 w2.1
+
+end
+
 section Alter
 
 theorem isEmpty_alter_eq_isEmpty_erase [TransCmp cmp] (h : t.WF) {k : α}
