src/Std/Data/TreeSet/Raw/Lemmas.lean
@@ -811,6 +811,21 @@ theorem isEmpty_inter_iff [TransCmp cmp] (h₁ : t₁.WF) (h₂ : t₂.WF) :
 
 end Inter
 
+section
+variable {m₁ m₂ : Raw α cmp}
+
+theorem Equiv.beq [TransCmp cmp] (h₁ : m₁.WF) (h₂ : m₂.WF) : m₁ ~m m₂ → beq m₁ m₂ := fun hyp =>
+  @TreeMap.Raw.Const.Equiv.beq _ cmp _ m₁.1 m₂.1 _ _ _ h₁ h₂ hyp.1
+
+theorem Equiv_of_beq_eq_true [TransCmp cmp] [LawfulEqCmp cmp] (h₁ : m₁.WF) (h₂ : m₂.WF) : m₁ == m₂ → m₁ ~m m₂ := fun hyp =>
+  ⟨@TreeMap.Raw.Const.Equiv_of_beq_eq_true α cmp _ m₁.1 m₂.1 _ _ _ _ h₁.1 h₂.1 hyp⟩
+
+theorem Equiv.beq_congr [TransCmp cmp] [LawfulEqCmp cmp] {m₃ m₄ : Raw α cmp} (h₁ : m₁.WF) (h₂ : m₂.WF) (h₃ : m₃.WF) (h₄ : m₄.WF) :
+    m₁ ~m m₃ → m₂ ~m m₄ → (m₁ == m₂) = (m₃ == m₄) := fun hyp1 hyp2 =>
+  @TreeMap.Raw.Const.Equiv.beq_congr α cmp _ m₁.1 m₂.1 _ _ _ m₃.1 m₄.1 h₁.1 h₂.1 h₃.1 h₄.1 hyp1.1 hyp2.1
+
+end
+
 section monadic
 
 variable {δ : Type w} {m : Type w → Type w'}
